

In[1]:=  $la = m * ht^2 / 2 - k * h^2 / 2$

Out[1]=  $-\frac{h^2 k}{2} + \frac{ht^2 m}{2}$

In[2]:=  $q = D[la, ht]$

Out[2]=  $ht m$

In[3]:=  $f = D[la, h]$

Out[3]=  $-h k$

In[4]:=  $s = q /. \{ht \rightarrow D[h[t], t], h \rightarrow h[t]\}$

Out[4]=  $m h'[t]$

In[5]:=  $c = f /. \{ht \rightarrow D[h[t], t], h \rightarrow h[t]\}$

Out[5]=  $-k h[t]$

In[6]:=  $EL = c - D[s, t]$

Out[6]=  $-k h[t] - m h''[t]$

In[7]:=  $la = m * L^2 * ht^2 / 2 - m * g * L * (1 - Cos[h])$

Out[7]=  $\frac{1}{2} ht^2 L^2 m - g L m (1 - Cos[h])$

In[8]:=  $q = D[la, ht]$

Out[8]=  $ht L^2 m$

In[9]:=  $s = q /. \{ht \rightarrow D[h[t], t], h \rightarrow h[t]\}$

Out[9]=  $L^2 m h'[t]$

In[10]:=  $dl = D[la, h]$

Out[10]=  $-g L m Sin[h]$

In[11]:=  $c = D[la, h] /. \{ht \rightarrow h'[t], h \rightarrow h[t]\}$

Out[11]=  $-g L m Sin[h[t]]$

In[12]:=  $EL = c - D[s, t]$

Out[12]=  $-g L m Sin[h[t]] - L^2 m h''[t]$

In[13]:=  $EL = Simplify[EL / (m * L)]$

Out[13]=  $-g Sin[h[t]] - L h''[t]$

```
In[19]:= w[la_] := Module[{q, f, o, d, c, s, r, EL},
  q = D[la, ht]; f = D[la, h]; o = D[la, htt];
  d = {htt → D[h[t], {t, 2}], ht → D[h[t], t], h → ht[t]};
  c = f /. d;
  s = q /. d;
  r = o /. d;
  EL = c - D[s, t] + D[r, {t, 2}];
  EL]
```

```
In[20]:= w[la]
```

```
Out[20]=
  -g L m Sin[ht[t]] - L^2 m h''[t]
```